Swap program and address in the definition of closure

TM/LM/Definitions.v
@@ -4,6 +4,6 @@ Require Import TM.Code.CodeTM.
 Inductive Tok := varT (n :nat) | appT | lamT | retT.
 Definition Pro := list Tok.
 Definition HAd : Type := nat.
-Definition HClos : Type := Pro * HAd.
+Definition HClos : Type := HAd * Pro.
 Definition HEnt : Type := option (HClos * HAd).
 Definition Heap : Type := list HEnt.
