TM/LM/HeapTM.v
@@ -19,18 +19,18 @@ Definition sigPro := sigList sigTok.
 Instance Encode_Prog : codable sigPro Pro := _.
 Definition sigPro_fin := FinType(EqType sigPro).
 
-Definition sigHClos := sigPair sigPro sigHAd.
-Instance Encode_HClos : codable (FinType (EqType sigHClos)) HClos := _.
+Definition sigHClos := sigPair sigHAd sigPro.
 Definition sigHClos_fin := FinType(EqType sigHClos).
+Instance Encode_HClos : codable sigHClos HClos := _.
 
 Definition sigHEnt' := sigPair sigHClos sigHAd.
-Instance Encode_HEnt' : codable (FinType (EqType sigHEnt')) (HClos*HAd) := _.
+Instance Encode_HEnt' : codable (sigHEnt') (HClos*HAd) := _.
 Definition sigHEnt'_fin := FinType(EqType sigHEnt').
 
 Definition sigHEnt := sigOption sigHEnt'.
-Instance Encode_HEnt : codable (FinType (EqType sigHEnt)) HEnt := _.
+Instance Encode_HEnt : codable (sigHEnt) HEnt := _.
 Definition sigHEnt_fin := FinType(EqType sigHEnt).
 
 Definition sigHeap := sigList sigHEnt.
-Instance Encode_Heap : codable (FinType (EqType sigHeap)) Heap := _.
+Instance Encode_Heap : codable (sigHeap) Heap := _.
 Definition sigHeap_fin := FinType(EqType sigHeap).
